renamed def to theorem

LeanCourse/StorageToMemory.lean
@@ -26,7 +26,7 @@ open Value
 @[simp] def copySt (mem : Memory α β γ δ) (id : δ) (st : Value α β γ) (wf : isStruct st) : Memory α β γ δ :=
   copyStAux (add mem id) ⟨id, []⟩ st wf
 
-def not_suff_imp_not_cons_suff (l1 l2 : List α) (x : α) :
+theorem not_suff_imp_not_cons_suff (l1 l2 : List α) (x : α) :
   ¬ (l1 <:+ l2) → ¬ (x :: l1 <:+ l2) := by
   intro h1 h2
   apply h1
@@ -34,7 +34,7 @@ def not_suff_imp_not_cons_suff (l1 l2 : List α) (x : α) :
   aesop
 
 
-def readSkip [DecidableEq β] [DecidableEq γ] [DecidableEq δ] [Inhabited α]
+theorem readSkip [DecidableEq β] [DecidableEq γ] [DecidableEq δ] [Inhabited α]
   (mem : Memory α β γ δ) (pId pIdR : δ) (st : Value α β γ) (fxsL fxsR : List (β ⊕ γ)) (fld : β ⊕ γ)
   (wf : isStruct st) (pIdDiff : ¬pId = pIdR ⊕' pId = pIdR ×' ¬ fxsL <:+ (fld :: fxsR))
   : read (copyStAux mem ⟨pId, fxsL⟩ st wf) ⟨ pIdR , fxsR ⟩ fld = read mem ⟨ pIdR, fxsR⟩ fld :=
@@ -78,7 +78,7 @@ inductive SameVal {α β γ δ : Type} : ValT α β γ δ → Value α β γ →
 
 open SameVal
 
-def readFind [DecidableEq β] [DecidableEq γ] [DecidableEq δ] [Inhabited α]
+theorem readFind [DecidableEq β] [DecidableEq γ] [DecidableEq δ] [Inhabited α]
   (mem : Memory α β γ δ) (id : δ) (st : Value α β γ) (fxs : List (β ⊕ γ)) (f : β) (wf : isStruct st)
   : SameVal (read (copySt mem id st wf) ⟨id, []⟩ (inl f)) (select st (inl f)) :=
   match st with
@@ -107,7 +107,7 @@ def readFind [DecidableEq β] [DecidableEq γ] [DecidableEq δ] [Inhabited α]
     . constructor
     . apply readFindd
 
-def skipIdRead [DecidableEq β] [DecidableEq γ] [DecidableEq δ] [Inhabited α]
+theorem skipIdRead [DecidableEq β] [DecidableEq γ] [DecidableEq δ] [Inhabited α]
   (mem : Memory α β γ δ) (idC idR : IdT β γ δ) (st : Value α β γ) (fld : γ) (wf : isStruct st)
   : read (copyStAux mem idC st wf) idR (inr fld) = read mem idR (inr fld) :=
   match st with
@@ -124,7 +124,7 @@ def skipIdRead [DecidableEq β] [DecidableEq γ] [DecidableEq δ] [Inhabited α]
     have _ := skipIdRead (copyStAux mem idC st wfIn) ⟨idC.1, inr id :: idC.2⟩ idR v fld (structInsideR wf)
     aesop
 
-def readGetId [DecidableEq β] [DecidableEq γ] [DecidableEq δ] [Inhabited α]
+theorem readGetId [DecidableEq β] [DecidableEq γ] [DecidableEq δ] [Inhabited α]
   (mem : Memory α β γ δ) (pId : δ) (st : Value α β γ) (fxs : List (β ⊕ γ)) (fld : γ) (wf : isStruct st)
   : read (copySt mem pId st wf) ⟨pId, fxs⟩ (inr fld) = inr ⟨pId, inr fld :: fxs⟩ := by
   have h := skipIdRead (add mem pId) ⟨pId, []⟩ ⟨pId, fxs⟩ st fld wf
